[plotkin] Section 3 done: SECD machine implements CBV for closed tms

examples/lambda/plotkin1975/plotkinScript.sml
@@ -156,6 +156,7 @@ Inductive dumpTrans:
   dumpTrans (((Cl::S,E,[])::(S',E',C')::D'):Dump)
             (((Cl::S',E',C')::D'):Dump)
 [~Cvar:]
+  x ∈ FDOM E ⇒
   dumpTrans ((S,E,Tm (VAR x)::C)::D)
             (((E ' x)::S,E,C)::D)
 [~Cconst:]
@@ -198,7 +199,6 @@ Proof
   >- (Cases_on ‘a’ >> Cases_on ‘b’ >> gvs[constapply_def, AllCaseEqs()] >>
       simp[EXTENSION, EQ_IMP_THM])
 QED
-
 
 Definition Unload_def:
   Unload ([]:Dump) = NONE ∧
@@ -360,9 +360,12 @@ Proof
 QED
 
 Overload fmFV = “λapm bpm. supp (fm_pmact apm bpm)”
-Overload clFV = “supp (fmt_pmact cterm_pmact string_pmact)”
-Overload eFV =
-  “supp (fm_pmact string_pmact (fmt_pmact cterm_pmact string_pmact))”
+Overload clpmact = “fmt_pmact cterm_pmact string_pmact”
+Overload clFV = “supp clpmact”
+Overload clpm = “pmact clpmact”
+Overload env_pmact = “fm_pmact string_pmact clpmact”
+Overload eFV = “supp env_pmact”
+Overload envpm = “pmact env_pmact”
 Overload subpm = “fmpm string_pmact cterm_pmact”
 Overload subFV = “supp (fm_pmact string_pmact cterm_pmact)”
 
@@ -797,17 +800,44 @@ Proof
   simp[Once timed_eval_cases]
 QED
 
+Theorem NRC_dumpTrans_app[local]:
+  NRC dumpTrans t ((S,E,Tm(M @@ N)::C)::D) D' ⇔
+    t = 0 ∧ D' = ((S,E,Tm(M@@N)::C)::D) ∨
+    ∃t0. t = SUC t0 ∧ NRC dumpTrans t0 ((S,E,Tm N :: Tm M :: Ap :: C)::D) D'
+Proof
+  Cases_on ‘t’ >> simp[EQ_SYM_EQ] >>
+  simp[arithmeticTheory.NRC] >>
+  simp[SimpLHS, dumpTrans_cases]
+QED
+
+Theorem errorState_appC[simp]:
+  ¬errorState ((S,E,Tm(M @@ N)::C)::D)
+Proof
+  simp[errorState_def, Once dumpTrans_cases]
+QED
+
+fun pull P l =
+  case total (pluck P) l of NONE => l | SOME (x,rest) => x::rest
+
+Theorem shorter_NRC_paths_exist:
+  ∀m n x y. NRC R n x y ∧ m ≤ n ⇒ ∃y0. NRC R m x y0
+Proof
+  Induct_on ‘n’ >> simp[arithmeticTheory.NRC] >> Cases_on ‘m’ >> simp[] >>
+  simp[arithmeticTheory.NRC] >> metis_tac[]
+QED
+
 (* “Suppose E is a value environment and ⟨M∶E⟩ is a closure.
     If Real(⟨M∶E⟩) has no value at any t' ≤ t, then either for all
     S, E, C, D, with FV(C) ⊆ Dom(E), (S,E,M::C)::D hits an error state
     or else (S,E,M::C)::D ⇒^t D' for some D'” *)
-(*
+(* Plotkin refers to "lemma 1" a couple of times in the course of the
+   proof; he actually means lemma 2. *)
 Theorem lemma3_3:
   ∀t E M.
     1 ≤ t ∧ isVEnv E ∧ wf_Closure ⟨M∶E⟩ ∧
     (∀t' N. t' ≤ t ⇒ ¬timed_eval t' (Real⟨M∶E⟩) N) ⇒
     ∀S C D.
-      cstrsFV C ⊆ FDOM E ⇒
+      isDump ((S,E,C)::D) ⇒
       (∃t' D'. NRC dumpTrans t' ((S,E,Tm M::C)::D) D' ∧ errorState D') ∨
       (∃D'. NRC dumpTrans t ((S,E,Tm M::C)::D) D')
 Proof
@@ -820,8 +850,496 @@ Proof
     by (Cases_on ‘M’ using cterm_CASES >>
         gvs[Excl "wf_Closure_thm", Real_LAM] >>
         rename [‘Real ⟨ VAR v ∶ E⟩’] >>
+        gvs[] >>
         ‘∃cl. FLOOKUP E v = SOME cl’ by simp[flookup_thm] >>
         gvs[Real_VAR] >> gvs[flookup_thm] >>
         drule_all isVEnv_Real >> simp[]) >>
+  gvs[] >> dsimp[NRC_dumpTrans_app] >>
+  Cases_on ‘t’ >> gvs[] >> rename [‘_ < SUC t0’] >>
+  reverse $ Cases_on ‘1 ≤ t0’ >> gvs[arithmeticTheory.NOT_LE] >>
+  reverse $ Cases_on ‘∃t2 N₂. t2 ≤ t0 ∧ timed_eval t2 (Real ⟨ M₂ ∶ E ⟩) N₂’
+  >- (gvs[] >>
+      CONV_TAC (
+        LAND_CONV $ RESORT_EXISTS_CONV (
+          pull (fn t => type_of t = numSyntax.num)
+        )
+      ) >> first_x_assum irule >> simp[] >> metis_tac[]) >>
   gvs[] >>
+  drule_at (Pat ‘timed_eval _ _ _’) lemma3_2 >> simp[SF CONJ_ss] >>
+  ‘cstrsFV (Tm M₁::Ap::C) ⊆ FDOM E’ by simp[] >>
+  disch_then (pop_assum o mp_then Any mp_tac) >>
+  disch_then $ drule_all_then strip_assume_tac >>
+  rename [‘NRC dumpTrans t2' ((S,E,Tm M₂ :: Tm M₁ :: Ap :: C)::D) (_::_)’] >>
+  Cases_on ‘t0 ≤ t2'’
+  >- metis_tac[shorter_NRC_paths_exist] >>
+  gvs[arithmeticTheory.NOT_LE] >>
+  reverse $ Cases_on
+      ‘∃nt N₁. nt ≤ t0 - t2' ∧ timed_eval nt (Real ⟨ M₁ ∶ E ⟩) N₁’
+  >- (gvs[DECIDE “¬p ∨ q ⇔ p ⇒ q”] >>
+      first_x_assum (pop_assum o mp_then Any mp_tac) >> simp[] >>
+      ‘cstrsFV (Ap::C) ⊆ FDOM E’ by simp[] >>
+      disch_then (pop_assum o mp_then Any mp_tac) >>
+      rename [‘isVClosure ⟨ M₂' ∶ E₂' ⟩’] >>
+      ‘∀cl. MEM cl (⟨ M₂' ∶ E₂'⟩ :: S) ⇒ wf_Closure cl’
+        by gvs[isVClosure_thm, DISJ_IMP_THM] >>
+      disch_then (drule_all_then strip_assume_tac)
+      >- metis_tac[arithmeticTheory.NRC_ADD_I] >>
+      ‘t2' + (t0 - t2') = t0’ by simp[] >>
+      metis_tac[arithmeticTheory.NRC_ADD_I]) >>
+  pop_assum (qx_choosel_then [‘t1’, ‘N₁’] strip_assume_tac) >>
+  first_assum (mp_then Any mp_tac lemma3_2) >> simp[] >>
+  rename [‘isVClosure ⟨ M₂' ∶ E₂' ⟩’] >>
+  ‘∀cl. MEM cl (⟨ M₂' ∶ E₂'⟩ :: S) ⇒ wf_Closure cl’
+    by gvs[isVClosure_thm, DISJ_IMP_THM] >>
+  disch_then (pop_assum o mp_then Any mp_tac) >> simp[SF SFY_ss] >>
+  ‘cstrsFV (Ap::C) ⊆ FDOM E’ by simp[] >>
+  disch_then (pop_assum o mp_then Any mp_tac) >>
+  disch_then $ drule_all_then strip_assume_tac >> gvs[] >>
+  rename [‘NRC _ t1' _ ((⟨ M₁' ∶ E₁' ⟩ :: ⟨ M₂' ∶ E₂' ⟩ :: _, _, _)::_)’] >>
+  Cases_on ‘t0 - t2' ≤ t1'’
+  >- (‘t2' + (t0 - t2') = t0’ by simp[] >>
+      disj2_tac >> pop_assum (SUBST1_TAC o SYM) >>
+      irule_at Any arithmeticTheory.NRC_ADD_I >>
+      first_assum $ irule_at Any >>
+      metis_tac[shorter_NRC_paths_exist]) >>
+  gvs[arithmeticTheory.NOT_LE] >>
+  Cases_on ‘∃x M₃. M₁' = LAM x M₃’
+  >- (gvs[] >>
+      ‘dumpTrans ((⟨ LAM x M₃ ∶ E₁' ⟩ :: ⟨ M₂' ∶ E₂' ⟩ :: S,
+                   E, Ap::C)::D)
+                 (([],E₁' |+ (x, ⟨ M₂' ∶ E₂' ⟩), [Tm M₃])::(S,E,C)::D)’
+        by (simp[Once dumpTrans_cases] >> irule_at Any EQ_REFL >> simp[]) >>
+      Cases_on ‘t0 = t2' + t1' + 1’
+      >- (disj2_tac >> pop_assum SUBST_ALL_TAC >>
+          irule_at Any arithmeticTheory.NRC_ADD_I >>
+          irule_at Any arithmeticTheory.NRC_ADD_I >>
+          simp[] >> rpt (first_assum $ irule_at Any)) >>
+      qabbrev_tac ‘E₃' = E₁' |+ (x, ⟨ M₂' ∶ E₂' ⟩)’ >>
+      reverse $ Cases_on ‘∃t3 N₃. t3 ≤ t0 - t1' - t2' - 1 ∧
+                                  timed_eval t3 (Real ⟨ M₃ ∶ E₃' ⟩) N₃’
+      >- (gvs[DECIDE “¬p ∨ q ⇔ p ⇒ q”] >>
+          first_x_assum (pop_assum o mp_then Any mp_tac) >>
+          simp[Abbr‘E₃'’, isVClosure_thm, DISJ_IMP_THM, FORALL_AND_THM,
+               FAPPLY_FUPDATE_THM] >>
+          ‘cFV M₃ ⊆ x INSERT FDOM E₁' ∧ cFV M₂' ⊆ FDOM E₂' ∧
+           (∀s. s ∈ FDOM E₂' ⇒ wf_Closure (E₂' ' s))’
+            by (gvs[isVClosure_thm] >> ASM_SET_TAC[]) >>
+          simp[] >>
+          ‘cstrsFV [] ⊆ x INSERT FDOM E₁'’ by simp[] >>
+          disch_then (drule_at (Pat ‘cstrsFV _ ⊆ _’)) >>
+          ‘isDump ((S,E,C)::D)’ by simp[flookup_thm] >>
+          disch_then (pop_assum o mp_then Any mp_tac) >>
+          disch_then (qspec_then ‘[]’ mp_tac) >> simp[] >>
+          impl_tac
+          >- (gvs[isVClosure_thm] >>
+              gvs[cj 2 isVClosure_cases, DOMSUB_FAPPLY_THM] >>
+              simp[flookup_thm, DISJ_IMP_THM, FAPPLY_FUPDATE_THM,
+                   FORALL_AND_THM] >>
+              rw[]) >>
+          strip_tac
+          >- (disj1_tac >> irule_at Any arithmeticTheory.NRC_ADD_I >>
+              first_assum $ irule_at (Pat ‘NRC _ _ (_::_) _’) >>
+              irule_at Any arithmeticTheory.NRC_ADD_I >>
+              first_assum $ irule_at (Pat ‘NRC _ _ (_::_) _’) >>
+              irule_at Any (iffRL $ cj 2 arithmeticTheory.NRC) >>
+              first_assum $ irule_at (Pat ‘dumpTrans _ _’) >>
+              metis_tac[]) >>
+          disj2_tac >>
+          ‘t0 = (t2' + t1' + 1) + (t0 - (t1' + t2' + 1))’ by simp[] >>
+          pop_assum SUBST1_TAC >> irule_at Any arithmeticTheory.NRC_ADD_I >>
+          irule_at Any arithmeticTheory.NRC_ADD_I >>
+          irule_at Any arithmeticTheory.NRC_ADD_I >> simp[] >> metis_tac[]) >>
+      gvs[] >>
+      ‘t1 + t2 + t3 + 1 ≤ SUC t0’ by simp[] >>
+      ‘F’ suffices_by simp[] >>
+      first_x_assum (pop_assum o mp_then Any mp_tac) >>
+      simp_tac bool_ss [] >>
+      qexists ‘N₃’ >>
+      irule timed_eval_app_tm >>
+      first_assum $ irule_at Any >>
+      ‘Real ⟨LAM x M₃ ∶ E₁'⟩ = LAM x (Real ⟨M₃ ∶ E₁' \\ x⟩)’
+        by (irule Real_LAM >> gvs[isVClosure_thm]) >> gvs[] >>
+      first_assum $ irule_at Any >>
+      dep_rewrite.DEP_REWRITE_TAC[GSYM lemma1_0] >> conj_tac
+      >- gvs[isVClosure_thm] >>
+      simp[Abbr‘E₃'’]) >>
+  Cases_on ‘∃a b N. M₁' = CONST a ∧ M₂' = CONST b ∧ constapply a b = SOME N’
+  >- (gvs[] >>
+      ‘t1 + t2 + 1 ≤ SUC t0’ by simp[] >>
+      ‘F’ suffices_by simp[] >>
+      first_x_assum (pop_assum o mp_then Any mp_tac) >>
+      simp_tac bool_ss [] >> qexists ‘N’ >>
+      irule timed_eval_app_const >> metis_tac[]) >>
+  disj1_tac >>
+  irule_at Any arithmeticTheory.NRC_ADD_I >>
+  first_assum $ irule_at Any >>
+  first_assum $ irule_at Any >>
+  simp[errorState_def]>> conj_tac
+  >- (simp[Once dumpTrans_cases] >> gvs[]) >>
+  Cases_on ‘D’ >> simp[Unload_def]
+QED
+
+Theorem Unload_EQ_SOME:
+  Unload D = SOME M ⇔
+  ∃Cl. D = [([Cl], FEMPTY, [])] ∧ M = Real Cl
+Proof
+  Cases_on ‘D’>> simp[Unload_def] >> rename [‘Unload (sec::rest)’] >>
+  Cases_on ‘rest’ >> simp[Unload_def] >> PairCases_on ‘sec’ >>
+  Cases_on ‘sec0’ >> simp[Unload_def] >>
+  Cases_on ‘sec2’ >> simp[Unload_def] >>
+  rename [‘Unload [(s1::rests,_)]’] >>
+  Cases_on ‘rests’ >> simp[Unload_def] >>
+  metis_tac[]
+QED
+
+Theorem dumpTrans_nf:
+  Unload D2 = SOME N ⇒ ∀D'. ¬dumpTrans D2 D'
+Proof
+  simp[Unload_EQ_SOME] >> rw[] >>
+  simp[Once dumpTrans_cases]
+QED
+
+Theorem R_det_RTC_det:
+  (∀x y z. R x y ∧ R x z ⇒ y = z) ⇒
+  ∀a b c. R꙳ a b ∧ R꙳ a c ∧ (∀b'. ¬R b b') ∧ (∀c'. ¬R c c') ⇒
+          b = c
+Proof
+  strip_tac >> Induct_on ‘RTC’ >> rw[]
+  >- (qpat_x_assum ‘R꙳ _ _’ mp_tac >> simp[Once relationTheory.RTC_CASES1]) >>
+  rename [‘b = c (* g *)’, ‘R꙳ a c’] >> qpat_x_assum ‘R꙳ a c’ mp_tac >>
+  simp[Once relationTheory.RTC_CASES1] >> rw[] >- gvs[] >>
+  metis_tac[]
+QED
+
+Definition raw_controlpm_def[simp]:
+  raw_controlpm π Ap = Ap ∧
+  raw_controlpm π (Tm t) = Tm (ctpm π t)
+End
+
+Definition control_pmact_def:
+  control_pmact = mk_pmact raw_controlpm
+End
+
+Theorem controlpm_def:
+  pmact control_pmact = raw_controlpm
+Proof
+  simp[GSYM pmact_bijections, control_pmact_def] >>
+  simp[is_pmact_def] >> rw[]
+  >- (Cases_on ‘x’ >> simp[])
+  >- (Cases_on ‘x’ >> simp[pmact_append]) >>
+  simp[FUN_EQ_THM] >> Cases >> simp[] >>
+  metis_tac[pmact_permeq]
+QED
+
+Theorem controlpm_thm[simp] = REWRITE_RULE[SYM controlpm_def] raw_controlpm_def
+
+Overload dump_pmact = “list_pmact (pair_pmact (list_pmact clpmact)
+                   (pair_pmact env_pmact (list_pmact control_pmact)))”
+
+(* mixture of invariant and alpha-equivalence like correspondence *)
+Definition dumpEQ_def:
+  dumpEQ d1 d2 ⇔
+    LIST_REL (λ(s1,e1,cs1) (s2,e2,cs2).
+                isVEnv e1 ∧ isVEnv e2 ∧
+                cstrsFV cs1 ⊆ FDOM e1 ∧ cstrsFV cs2 ⊆ FDOM e2 ∧
+                (∀cl. MEM cl s1 ⇒ isVClosure cl) ∧
+                (∀cl. MEM cl s2 ⇒ isVClosure cl) ∧
+                MAP Real s1 = MAP Real s2 ∧
+                LIST_REL (λc1 c2. c1 = Ap ∧ c2 = Ap ∨
+                                  ∃t1 t2. c1 = Tm t1 ∧ c2 = Tm t2 ∧
+                                          Real ⟨ t1 ∶ e1 ⟩ = Real ⟨ t2 ∶ e2 ⟩)
+                         cs1 cs2)
+             d1 d2 ∧
+    0 < LENGTH d1 ∧
+    FST (SND (LAST d1)) = FEMPTY ∧
+    FST (SND (LAST d2)) = FEMPTY
+End
+
+val _ = temp_set_mapped_fixity{
+  fixity = Infix(NONASSOC, 450),
+  term_name = "dumpEQ",
+  tok = "≈"
+  }
+
+Theorem constapply_ground:
+  constapply a b = SOME M ⇒ closed M
+Proof
+  map_every Cases_on [‘a’, ‘b’] >> simp[constapply_def] >> rw[] >> simp[] >>
+  simp[EXTENSION] >> simp[EQ_IMP_THM]
+QED
+
+Theorem constapply_value:
+  constapply a b = SOME M ⇒ is_abs M ∨ is_const M
+Proof
+  map_every Cases_on [‘a’, ‘b’] >> simp[constapply_def] >> rw[] >> simp[]
+QED
+
+Theorem clFV_SUBSET_eFV:
+  k ∈ FDOM fm ∧ a ∈ clFV (fm ' k) ⇒ a ∈ eFV fm
+Proof
+  simp[fmap_supp, supp_setpm, DECIDE “¬p ∨ q ⇔ p ⇒ q”, PULL_EXISTS] >>
+  strip_tac >>
+  ‘fm ' k ∈ FRANGE fm’ by (simp[TO_FLOOKUP, NoAsms] >> simp[flookup_thm] >>
+                           metis_tac[]) >>
+  metis_tac[]
+QED
+
+Theorem cFV_Real_SUBSET_clFV:
+  ∀Cl z. z ∈ cFV (Real Cl) ⇒ z ∈ clFV Cl
+Proof
+  simp[Real_def] >> Induct_on ‘Cl’ using ft_ind >>
+  simp[fmtreerec_thm, supp_fmtpm] >> gen_tac >> strip_tac >>
+  CCONTR_TAC >> qpat_x_assum ‘z ∈ cFV _’ mp_tac >> simp[] >>
+  irule fresh_ssub >> gvs[] >> gen_tac >> rpt strip_tac >>
+  first_x_assum drule_all >> metis_tac[clFV_SUBSET_eFV]
+QED
+
+Theorem Real_LAM_NEQ_APP[simp]:
+  Real ⟨ LAM v M ∶ E⟩ ≠ N @@ P
+Proof
+  simp[Real_def, fmtreerec_thm] >>
+  rename [‘LAM v M’, ‘_ o_f E’] >>
+  Q_TAC (NEW_TAC "z") ‘{v} ∪ cFV M ∪ eFV E’ >>
+  ‘LAM v M = LAM z (ctpm[(z,v)] M)’ by simp[ctpm_ALPHA] >>
+  simp[] >> rpt gen_tac >>
+  qmatch_abbrev_tac ‘FM ' _ ≠ _’ >>
+  ‘z ∉ FDOM FM’ by (simp[Abbr‘FM’] >> gvs[fmap_supp]) >>
+  ‘∀k. k ∈ FDOM FM ⇒ z ∉ cFV (FM ' k)’ suffices_by
+    (strip_tac >> simp[ssub_thm]) >>
+  rpt strip_tac >>
+  gvs[Abbr‘FM’, GSYM Real_def] >>
+  metis_tac[cFV_Real_SUBSET_clFV, clFV_SUBSET_eFV]
+QED
+
+Theorem Real_LAM_NEQ_CONST[simp]:
+  Real ⟨ LAM v M ∶ E⟩ ≠ CONST c
+Proof
+  simp[Real_def, fmtreerec_thm] >>
+  rename [‘LAM v M’, ‘_ o_f E’] >>
+  Q_TAC (NEW_TAC "z") ‘{v} ∪ cFV M ∪ eFV E’ >>
+  ‘LAM v M = LAM z (ctpm[(z,v)] M)’ by simp[ctpm_ALPHA] >>
+  simp[] >> rpt gen_tac >>
+  qmatch_abbrev_tac ‘FM ' _ ≠ _’ >>
+  ‘z ∉ FDOM FM’ by (simp[Abbr‘FM’] >> gvs[fmap_supp]) >>
+  ‘∀k. k ∈ FDOM FM ⇒ z ∉ cFV (FM ' k)’ suffices_by
+    (strip_tac >> simp[ssub_thm]) >>
+  rpt strip_tac >>
+  gvs[Abbr‘FM’, GSYM Real_def] >>
+  metis_tac[cFV_Real_SUBSET_clFV, clFV_SUBSET_eFV]
+QED
+
+Theorem dumpTrans_det:
+  ∀a1 a2 b c. dumpEQ a1 a2 ∧ dumpTrans a1 b ∧ dumpTrans a2 c ⇒ dumpEQ b c
+Proof
+  Induct_on ‘dumpTrans’ >> rpt conj_tac >>
+  simp[Once dumpTrans_cases] >> rw[] >>
+  gvs[dumpEQ_def, fmtpm_thm, Real_VAR, AllCaseEqs(), flookup_thm,
+      DISJ_IMP_THM, FORALL_AND_THM, cj 2 isVClosure_cases,
+      isVClosure_wf_Closure] >> rpt strip_tac >>~-
+  ([‘_ = FEMPTY (* g *)’, ‘LIST_REL _ (D1 : Dump) (D2 : Dump)’],
+   Cases_on ‘D1’ >> Cases_on ‘D2’ >> gvs[]) >>~-
+  ([‘isVClosure (_ ' k) (* g *)’],
+   rw[FAPPLY_FUPDATE_THM] >> gvs[isVClosure_thm] >>
+   gvs[cj 2 isVClosure_cases]) >>~-
+  ([‘isVClosure _ (* g *)’],
+   simp[isVClosure_thm] >> simp[cj 2 isVClosure_cases, isVClosure_wf_Closure] >>
+   metis_tac [constapply_ground, constapply_value]) >>~-
+  ([‘v ∈ FDOM E (* a *)’],
+   drule_at (Pat ‘v ∈ FDOM E’) isVEnv_Real >>
+   simp[cj 2 isVClosure_cases]) >>~-
+  ([‘_ ⊆ _ (* g *)’], gvs[isVClosure_thm] >> ASM_SET_TAC[]) >~
+  [‘Real ⟨LAM v1 M1 ∶ E1⟩ = Real ⟨LAM v2 M2 ∶ E2⟩’] >>
+  ‘wf_Closure ⟨LAM v1 M1 ∶ E1⟩ ∧ wf_Closure ⟨LAM v2 M2 ∶ E2⟩’
+    by simp[isVClosure_wf_Closure, Excl "wf_Closure_thm"] >>
+  ‘Real ⟨LAM v1 M1 ∶ E1⟩ = LAM v1 (Real⟨M1 ∶ E1 \\ v1⟩) ∧
+   Real ⟨LAM v2 M2 ∶ E2⟩ = LAM v2 (Real⟨M2 ∶ E2 \\ v2⟩)’
+    by simp[Real_LAM, IgnAsm ‘Real _ = Real _’] >>
+  ntac 2 (pop_assum $ mp_then Any mp_tac lemma3_1) >>
+  simp[Excl "wf_Closure_thm"] >>
+  rename [‘Real Cl1 = Real Cl2’, ‘E1 |+ (v1,Cl1)’, ‘E2 |+ (v2,Cl2)’] >>
+  Cases_on ‘Cl1’ using fmaptree_nchotomy >>
+  Cases_on ‘Cl2’ using fmaptree_nchotomy >>
+  rename [‘Real ⟨N1 ∶ E1'⟩ = Real⟨N2∶E2'⟩’,
+          ‘E1 |+ (v1,⟨N1 ∶ E1'⟩)’, ‘E2 |+ (v2,⟨N2∶E2'⟩)’] >>
+  simp[isVClosure_wf_Closure, Excl "wf_Closure_thm"] >> rpt strip_tac >>
+  qpat_x_assum ‘Real ⟨LAM _ _ ∶ _⟩ = Real _’ mp_tac >>
+  simp[Real_LAM] >> rw[LAM_eq_thm] >> simp[] >>
+  simp[ctpm_subst_out] >>
+  simp[ctpm_fresh, Excl "wf_Closure_thm", wf_Closure_Real_ground,
+       isVClosure_wf_Closure] >>
+  irule ctpm_fresh >> simp[cFV_SUB] >> rw[] >>
+  simp[Excl "wf_Closure_thm", wf_Closure_Real_ground,
+       isVClosure_wf_Closure]
+QED
+
+Theorem dumpEQ_SYM:
+  dumpEQ d1 d2 ⇔ dumpEQ d2 d1
+Proof
+  ‘∀d1 d2. dumpEQ d1 d2 ⇒ dumpEQ d2 d1’ suffices_by metis_tac[] >>
+  simp[dumpEQ_def] >> rpt strip_tac
+  >- (irule listTheory.EVERY2_sym >> first_assum $ irule_at Any >>
+      simp[pairTheory.FORALL_PROD] >> rw[] >>
+      irule listTheory.EVERY2_sym >> first_assum $ irule_at Any>>
+      simp[PULL_EXISTS, DISJ_IMP_THM, FORALL_AND_THM]) >>
+  metis_tac[listTheory.LIST_REL_LENGTH]
+QED
+
+Theorem isVClosure_noncases[simp]:
+  ¬isVClosure ⟨ VAR v ∶ E ⟩ ∧ ¬isVClosure ⟨ M @@ N ∶ E ⟩
+Proof
+  simp[isVClosure_thm]
+QED
+
+Theorem dumpEQ_preserves_nf:
+  dumpEQ d1 d2 ⇒ (nf dumpTrans d1 ⇔ nf dumpTrans d2)
+Proof
+  ‘∀d1 d2. dumpEQ d1 d2 ∧ nf dumpTrans d1 ⇒ nf dumpTrans d2’
+    suffices_by metis_tac[dumpEQ_SYM] >>
+  simp[relationTheory.nf_def] >>
+  ‘∀d1 d2 y. dumpEQ d1 d2 ∧ dumpTrans d2 y ⇒ ∃y. dumpTrans d1 y’
+    suffices_by metis_tac[] >>
+  Induct_on ‘dumpTrans’ >>
+  simp[dumpEQ_def, pairTheory.FORALL_PROD, pairTheory.EXISTS_PROD,
+       listTheory.MAP_EQ_CONS] >>
+  rw[] >>~-
+  ([‘Tm t1::_ (* sg *)’],
+   simp[dumpTrans_cases] >> simp[EXISTS_OR_THM] >>
+   rename [‘t = VAR _ ∧ _ ∈ _’] >> Cases_on ‘t’ using cterm_CASES >> gvs[] >>
+   irule_at Any EQ_REFL) >~
+  [‘((Shd::Stl,E,[])::_::_) (* sg *)’]
+  >- simp[dumpTrans_cases] >~
+  [‘Ap::_’, ‘Real ⟨ LAM v M ∶ E⟩ = Real Abs’]
+  >- (simp[dumpTrans_cases] >> simp[EXISTS_OR_THM] >>
+      Cases_on ‘Abs’ using fmaptree_nchotomy >>
+      simp[] >> rename [‘tm = LAM _ _ (* sg *)’] >>
+      Cases_on ‘tm’ using cterm_CASES >> gvs[DISJ_IMP_THM, FORALL_AND_THM] >>
+      irule_at Any EQ_REFL) >~
+  [‘Ap::_’, ‘CONST c1 = Real _’]
+  >- (simp[dumpTrans_cases] >> simp[EXISTS_OR_THM] >>
+      rename [‘cl1 = ⟨CONST _ ∶ _⟩ ∧ cl2 = ⟨CONST _ ∶ _⟩ ∧ _’] >>
+      Cases_on ‘cl1’ using fmaptree_nchotomy >>
+      Cases_on ‘cl2’ using fmaptree_nchotomy >> gvs[] >>
+      rename [‘t1 = CONST _ ∧ t2 = CONST _ ∧ _’] >>
+      Cases_on ‘t1’ using cterm_CASES >> Cases_on ‘t2’ using cterm_CASES >>
+      gvs[DISJ_IMP_THM, FORALL_AND_THM])
+QED
+
+Theorem RTC_dumpTrans_det:
+  ∀d1 d2 e1 e2.
+    dumpEQ d1 d2 ∧ dumpTrans꙳ d1 e1 ∧ dumpTrans꙳ d2 e2 ∧
+    nf dumpTrans e1 ∧ nf dumpTrans e2 ⇒
+    dumpEQ e1 e2
+Proof
+  Induct_on ‘RTC’ >> rw[] >> gvs[] >~
+  [‘dumpTrans꙳ d2 e2’, ‘d1 ≈ d2’, ‘nf dumpTrans e2’, ‘nf dumpTrans d1’]
+  >- (‘nf dumpTrans d2’ by metis_tac[dumpEQ_preserves_nf] >>
+      ‘e2 = d2’ suffices_by simp[] >>
+      qpat_x_assum ‘dumpTrans꙳ _ _’ mp_tac >>
+      simp[Once relationTheory.RTC_CASES1] >>
+      gvs[relationTheory.nf_def]) >~
+  [‘dumpTrans d1 dA’, ‘dumpTrans꙳ dA e1’, ‘d1 ≈ d2’, ‘dumpTrans꙳ d2 e2’,
+   ‘nf dumpTrans e2’]
+  >- (‘¬nf dumpTrans d1’ by simp[SF SFY_ss, relationTheory.nf_def] >>
+      ‘¬nf dumpTrans d2’ by metis_tac[dumpEQ_preserves_nf] >>
+      ‘d2 ≠ e2’ by (strip_tac >> gvs[]) >>
+      qpat_x_assum ‘dumpTrans꙳ d2 e2’ mp_tac >>
+      simp[Once relationTheory.RTC_CASES1] >> strip_tac >>
+      metis_tac[dumpTrans_det])
+QED
+
+Theorem dumpEQ_Load:
+  closed M ⇒ dumpEQ (Load M) (Load M)
+Proof
+  simp[dumpEQ_def, Load_def] >> simp[cj 2 isVClosure_cases]
+QED
+
+Theorem Eval_det:
+  closed M ∧ Eval M N1 ∧ Eval M N2 ⇒ N1 = N2
+Proof
+  simp[Eval_def] >> rpt strip_tac >>
+  rename [‘N1 = N2 (* g *)’, ‘Unload D1 = SOME N1’, ‘Unload D2 = SOME N2’] >>
+  gvs[Unload_EQ_SOME] >>
+  ‘Load M ≈ Load M’ by simp[dumpEQ_Load] >>
+  ‘∀Cl. nf dumpTrans [([Cl], FEMPTY, [])]’
+    by simp[relationTheory.nf_def, dumpTrans_cases] >>
+  dxrule_then (dxrule_then dxrule) RTC_dumpTrans_det >>
+  simp[dumpEQ_def]
+QED
+
+Theorem dumpTrans_succeeds_noerrors:
+  ∀n d1 d2 d N.
+    d1 ≈ d2 ∧ NRC dumpTrans n d1 d ∧ Unload d = SOME N ⇒
+    (∀t err. NRC dumpTrans t d2 err ⇒ ¬errorState err)
+Proof
+  simp[errorState_def] >> Induct_on ‘n’ >> simp[] >> rw[]
+  >- (‘nf dumpTrans d1’
+        by gvs[Unload_EQ_SOME,relationTheory.nf_def, dumpTrans_cases] >>
+      ‘nf dumpTrans d2’ by metis_tac[dumpEQ_preserves_nf] >>
+      Cases_on ‘t’ >> gvs[]
+      >- (gvs[Unload_EQ_SOME, dumpEQ_def] >> rename [‘Unload [sec] = NONE’] >>
+          PairCases_on ‘sec’ >> gvs[Unload_def]) >>
+      gvs[arithmeticTheory.NRC, relationTheory.nf_def]) >>
+  gvs[arithmeticTheory.NRC] >>
+  rename [‘dumpTrans d1 dA’, ‘d1 ≈ d2’]>>
+  ‘¬nf dumpTrans d1’ by simp[SF SFY_ss, relationTheory.nf_def] >>
+  ‘¬nf dumpTrans d2’ by metis_tac[dumpEQ_preserves_nf] >>
+  rename [‘Unload err = NONE’, ‘NRC _ m d2 err’] >>
+  Cases_on ‘m’ >> gvs[arithmeticTheory.NRC]
+  >- metis_tac[relationTheory.nf_def] >>
+  drule_all dumpTrans_det >> metis_tac[]
+QED
+
+Theorem dumpTrans_succeeds_nolater_transitions:
+  ∀n d1 d2 d N.
+    d1 ≈ d2 ∧ NRC dumpTrans n d1 d ∧ Unload d = SOME N ⇒
+    ∀m e. n < m ⇒ ¬NRC dumpTrans m d2 e
+Proof
+  Induct_on ‘n’ >> simp[] >> rw[]
+  >- (‘nf dumpTrans d1’ by gvs[Unload_EQ_SOME, relationTheory.nf_def,
+                               dumpTrans_cases] >>
+      ‘nf dumpTrans d2’ by metis_tac[dumpEQ_preserves_nf] >>
+      Cases_on ‘m’ >>
+      gvs[arithmeticTheory.NRC, relationTheory.nf_def]) >>
+  gvs[arithmeticTheory.NRC] >>
+  Cases_on ‘m’ >> gvs[arithmeticTheory.NRC] >>
+  metis_tac[dumpTrans_det]
+QED
+
+(* stated on p131: "For any program M, Eval_V(M) =_α eval_V(M)"
+   (programs are closed terms, first paragraph of §3:
+     "Its [ISWIM's] set of programs is just the set of closed terms")
 *)
+Theorem theorem3_1:
+  closed M ⇒ (Eval M N ⇔ eval M N)
+Proof
+  strip_tac >>
+  ‘wf_Closure ⟨ M ∶ FEMPTY ⟩’ by simp[] >>
+  ‘Real ⟨ M ∶ FEMPTY ⟩ = M’ by simp[Real_thm] >>
+  ‘(∀N. eval M N ⇒ Eval M N) ∧ ((∀N. ¬eval M N) ⇒ (∀N. ¬Eval M N))’
+    suffices_by (strip_tac >> reverse iff_tac >> simp[] >>
+                 Cases_on ‘∃N. eval M N’
+                 >- (gvs[] >> first_x_assum drule >> metis_tac[Eval_det]) >>
+                 metis_tac[]) >>
+  conj_tac
+  >- (simp[eval_timed_eval] >> rpt strip_tac >> rename [‘timed_eval t’] >>
+      ‘timed_eval t (Real ⟨ M ∶ FEMPTY ⟩) N’ by simp[] >>
+      dxrule_at (Pat ‘timed_eval _ _ _’) lemma3_2 >>
+      simp[isVClosure_thm] >>
+      disch_then $ qspecl_then [‘[]’, ‘[]’, ‘[]’] mp_tac >> simp[] >>
+      strip_tac >> gvs[Eval_def, Load_def] >>
+      irule_at Any arithmeticTheory.NRC_RTC >>
+      first_assum $ irule_at Any >> simp[Unload_def]) >>
+  CCONTR_TAC >> gvs[eval_timed_eval] >>
+  qpat_x_assum ‘Eval M N’ mp_tac >>
+  simp[Eval_def] >> rpt strip_tac >> gvs[Load_def] >>
+  drule_then strip_assume_tac arithmeticTheory.RTC_NRC >>
+  drule_then strip_assume_tac dumpTrans_nf >>
+  ‘wf_Closure ⟨ M ∶ FEMPTY ⟩’ by simp[] >>
+  drule_at_then (Pat ‘wf_Closure _’) assume_tac lemma3_3 >>
+  ‘isDump [([],FEMPTY,[])]’ by simp[isDump_def] >>
+  first_x_assum (dxrule_at Any) >> simp[isVClosure_thm] >>
+  rename [‘NRC dumpTrans n _ _’] >>
+  qexists ‘n + 1’ >> simp[] >> gvs[GSYM Load_def] >>
+  metis_tac[dumpTrans_succeeds_noerrors, dumpEQ_Load,
+            dumpTrans_succeeds_nolater_transitions, DECIDE “n < n + 1”]
+QED
